Anon3Assignment/Student.lean
@@ -16,4 +16,19 @@ def addElement (s : State) (n : Nat) : State :=
 def calculateMKAverage (s : State) : Int :=
   sorry
 
+def implementation : MKImplementation where
+  State := State
+  init := init
+  addElement := addElement
+  calculateMKAverage := calculateMKAverage
+
+theorem solution_is_correct
+    (m k : Nat)
+    (hm : 3 ≤ m)
+    (hk : 2 * k < m)
+    (ops : List Op) :
+    runImplementation implementation m k ops =
+      runBaseline m k ops := by
+  sorry
+
 end Anon3.Student
